src/program_proof/rsm/distx/action.v
@@ -1,0 +1,287 @@
+From Perennial.program_proof Require Import grove_prelude.
+(* TODO: remove this once invariance proof moved to their places. *)
+From Perennial.program_proof.rsm.pure Require Import list.
+From Perennial.program_proof.rsm.distx Require Import base.
+
+Definition head_commit (l : list action) (ts : nat) (wrs : dbmap) :=
+  head l = Some (ActCommit ts wrs).
+
+Definition head_read (l : list action) (ts : nat) (key : dbkey) :=
+  head l = Some (ActRead ts key).
+
+Definition no_commit (l : list action) (tid : nat) :=
+  ∀ wrs, ActCommit tid wrs ∉ l.
+
+Definition compatible (ts : nat) (wrs : dbmap) (a : action) :=
+  match a with
+  | ActCommit tsa wrsa => (tsa < ts)%nat ∨ (dom wrs) ∩ (dom wrsa) = ∅
+  | ActRead tsa key => (tsa ≤ ts)%nat ∨ key ∉ (dom wrs)
+  end.
+
+#[local]
+Instance compatible_dec ts wrs a : Decision (compatible ts wrs a).
+Proof. destruct a; simpl; apply _. Defined.
+
+Definition incompatible (ts : nat) (wrs : dbmap) (a : action) := not (compatible ts wrs a).
+
+Definition compatible_all (l : list action) (ts : nat) (wrs : dbmap) :=
+  Forall (compatible ts wrs) l.
+
+Definition incompatible_exists (l : list action) (ts : nat) (wrs : dbmap) :=
+  Exists (incompatible ts wrs) l.
+
+Lemma not_compatible_all_incompatible_exists l ts wrs :
+  not (compatible_all l ts wrs) ↔ incompatible_exists l ts wrs.
+Proof.
+  split; intros H.
+  - by apply not_Forall_Exists in H; last apply _.
+  - by apply Exists_not_Forall in H.
+Qed.
+
+(** A more natural definition of [first_commit] would be hiding [lp] and [ls]
+with exists, but and intuitively it says "the first commit action in [l] with
+timestamp [ts] is [ActCommit ts wrs]". However, [first_commit_incompatible]
+needs access to the first part of [l] (i.e., the one without any commit action
+of timestamp [ts], so we expose [lp] and [ls] as well. *)
+
+Definition first_commit (l lp ls : list action) (ts : nat) (wrs : dbmap) :=
+  l = lp ++ ls ∧
+  no_commit lp ts ∧
+  head ls = Some (ActCommit ts wrs).
+
+Definition first_commit_incompatible (l1 l2 : list action) (ts : nat) (wrs : dbmap) :=
+  ∃ lp ls,
+    first_commit l2 lp ls ts wrs ∧
+    incompatible_exists (l1 ++ lp) ts wrs.
+
+Definition first_commit_compatible (l : list action) (ts : nat) (wrs : dbmap) :=
+  ∃ lp ls,
+    first_commit l lp ls ts wrs ∧
+    compatible_all lp ts wrs.
+
+(* TODO: rename to [find_max_prefix_before_commit]. *)
+Fixpoint find_max_prefix (ts : nat) (lp ls : list action) : (list action * list action) :=
+  match ls with
+  | [] => (lp, ls)
+  | hd :: tl => match hd with
+              | ActCommit tshd _ => if decide (tshd = ts)
+                                   then (lp, ls)
+                                   else find_max_prefix ts (lp ++ [hd]) tl
+              | ActRead _ _ => find_max_prefix ts (lp ++ [hd]) tl
+              end
+  end.
+
+(* TODO: rename to [find_max_prefix_before_commit_spec]. *)
+Lemma spec_find_max_prefix ts lp ls :
+  ∃ ls1 ls2,
+    find_max_prefix ts lp ls = (lp ++ ls1, ls2) ∧
+    ls = ls1 ++ ls2 ∧
+    no_commit ls1 ts ∧
+    (ls2 = [] ∨ ∃ wrs, head ls2 = Some (ActCommit ts wrs)).
+Proof.
+  generalize dependent lp.
+  induction ls as [| a ls IH]; intros lp; simpl.
+  { exists [], [].
+    split; first by rewrite app_nil_r.
+    split; first done.
+    split.
+    { rewrite /no_commit. set_solver. }
+    by left.
+  }
+  destruct a as [tsa wrs | tsa key] eqn:Ha; rewrite -Ha; last first.
+  { destruct (IH (lp ++ [a])) as (ls1 & ls2 & Heq & Hls2 & Hnc & Hhead).
+    exists ([a] ++ ls1), ls2.
+    split; first by rewrite app_assoc Heq.
+    split; first set_solver.
+    split.
+    { intros wrsa.
+      rewrite not_elem_of_app.
+      split; [set_solver | done].
+    }
+    done.
+  }
+  case_decide as Htsa; last first.
+  { destruct (IH (lp ++ [a])) as (ls1 & ls2 & Heq & Hls2 & Hnc & Hhead).
+    exists ([a] ++ ls1), ls2.
+    split; first by rewrite app_assoc Heq.
+    split; first set_solver.
+    split.
+    { intros wrsa.
+      rewrite not_elem_of_app.
+      split; [set_solver | done].
+    }
+    done.
+  }
+  exists [], (a :: ls).
+  split; first by rewrite app_nil_r.
+  split; first by rewrite app_nil_l.
+  split.
+  { rewrite /no_commit. set_solver. }
+  right.
+  rewrite Ha Htsa.
+  by eauto.
+Qed.
+
+Inductive tcform :=
+(* no commit in the entire list of actions *)
+| NC
+(* first commit incompatible with some previous actions *)
+| FCI (wrs : dbmap)
+(* first commit compatible with some previous actions *)
+| FCC (wrs : dbmap).
+
+Definition peek (l : list action) (ts : nat) : tcform :=
+  let (lp, ls) := find_max_prefix ts [] l in
+  match head ls with
+  | None => NC
+  | Some a => match a with
+             | ActCommit _ wrs => if decide (compatible_all lp ts wrs)
+                                 then FCC wrs
+                                 else FCI wrs
+             | _ => NC (* impossible case *)
+             end
+  end.
+
+(* TODO: rename to [peek_spec]. *)
+Theorem spec_peek l ts :
+  match peek l ts with
+  | NC => no_commit l ts
+  | FCI wrs => first_commit_incompatible [] l ts wrs
+  | FCC wrs => first_commit_compatible l ts wrs
+  end.
+Proof.
+  unfold peek.
+  destruct (spec_find_max_prefix ts [] l) as (lp & ls & -> & Hl & Hnc & Hls).
+  destruct Hls as [Hls | [wrs Hls]].
+  { subst ls. by rewrite /= Hl app_nil_r. }
+  rewrite Hls.
+  case_decide as Hcomp.
+  { by exists lp, ls. }
+  { exists lp, ls. by rewrite -not_compatible_all_incompatible_exists. }
+Qed.
+
+(* TODO: move to invariance/read *)
+Lemma head_read_first_commit_compatible future ts tshd wrs keyhd :
+  head_read future tshd keyhd ->
+  first_commit_compatible future ts wrs ->
+  keyhd ∈ dom wrs ->
+  (tshd ≤ ts)%nat.
+Proof.
+  intros Hhr (lp & ls & (Happ & _ & Hhead) & Hcomp) Hnempty.
+  destruct (decide (lp = [])) as [-> | Hnnil].
+  { rewrite Happ /= /head_read Hhead in Hhr. inv Hhr. }
+  assert (Hlp : ActRead tshd keyhd ∈ lp).
+  { apply head_Some_elem_of.
+    rewrite (head_prefix _ future); [done | apply Hnnil |].
+    rewrite Happ.
+    by apply prefix_app_r.
+  }
+  rewrite /compatible_all Forall_forall in Hcomp.
+  specialize (Hcomp _ Hlp).
+  destruct Hcomp; [lia | contradiction].
+Qed.
+(* TODO: move to invariance/read *)
+
+(* TODO: move to invariance/commit *)
+Lemma head_commit_no_commit future ts wrs :
+  head_commit future ts wrs ->
+  no_commit future ts ->
+  False.
+Proof.
+  intros Hhc Hnc.
+  specialize (Hnc wrs).
+  by apply head_Some_elem_of in Hhc.
+Qed.
+
+Lemma head_commit_first_commit future lp ls ts wrs wrshd :
+  head_commit future ts wrshd ->
+  first_commit future lp ls ts wrs ->
+  wrshd = wrs.
+Proof.
+  intros Hhc (Happ & Hnc & Hhead).
+  destruct lp as [| x l]; last first.
+  { rewrite Happ /head_commit /= in Hhc.
+    inv Hhc.
+    specialize (Hnc wrshd).
+    set_solver.
+  }
+  rewrite Happ /= /head_commit Hhead in Hhc.
+  by inv Hhc.
+Qed.
+
+Lemma head_commit_first_commit_compatible future ts tshd wrs wrshd :
+  head_commit future tshd wrshd ->
+  first_commit_compatible future ts wrs ->
+  dom wrs ∩ dom wrshd ≠ ∅ ->
+  (tshd ≤ ts)%nat.
+Proof.
+  intros Hhc (lp & ls & (Happ & _ & Hhead) & Hcomp) Hnempty.
+  destruct (decide (lp = [])) as [-> | Hnnil].
+  { rewrite Happ /= /head_commit Hhead in Hhc. by inv Hhc. }
+  assert (Hlp : ActCommit tshd wrshd ∈ lp).
+  { apply head_Some_elem_of.
+    rewrite (head_prefix _ future); [done | apply Hnnil |].
+    rewrite Happ.
+    by apply prefix_app_r.
+  }
+  rewrite /compatible_all Forall_forall in Hcomp.
+  specialize (Hcomp _ Hlp).
+  destruct Hcomp; [lia | contradiction].
+Qed.
+
+Lemma no_commit_inv_commit l ts :
+  no_commit l ts ->
+  no_commit (tail l) ts.
+Proof. intros Hnc wrs. by apply not_elem_of_tail. Qed.
+
+Lemma first_commit_incompatible_inv_commit past future ts tshd wrs wrshd :
+  ts ≠ tshd ->
+  head_commit future tshd wrshd ->
+  first_commit_incompatible past future ts wrs ->
+  first_commit_incompatible (past ++ [ActCommit tshd wrshd]) (tail future) ts wrs.
+Proof.
+  intros Hne Hhead (lp & ls & (Happ & Hnc & Hheadls) & Hincomp).
+  assert (Hnnil : lp ≠ nil).
+  { intros Hlp. subst lp.
+    simpl in Happ. subst ls.
+    rewrite Hhead in Hheadls.
+    inv Hheadls.
+  }
+  exists (tail lp), ls.
+  split.
+  { split.
+    { rewrite Happ. apply tail_app_l, Hnnil. }
+    by split; first apply no_commit_inv_commit.
+  }
+  rewrite -app_assoc /=.
+  replace (_ :: _) with lp; first apply Hincomp.
+  rewrite -hd_error_tl_repr.
+  split; last done.
+  rewrite -Hhead.
+  apply head_prefix; first apply Hnnil.
+  rewrite Happ.
+  by apply prefix_app_r.
+Qed.
+
+Lemma first_commit_compatible_inv_commit future ts tshd wrs wrshd :
+  ts ≠ tshd ->
+  head_commit future tshd wrshd ->
+  first_commit_compatible future ts wrs ->
+  first_commit_compatible (tail future) ts wrs.
+Proof.
+  intros Hne Hhead (lp & ls & (Happ & Hnc & Hheadls) & Hincomp).
+  assert (Hnnil : lp ≠ nil).
+  { intros Hlp. subst lp.
+    simpl in Happ. subst ls.
+    rewrite Hhead in Hheadls.
+    inv Hheadls.
+  }
+  exists (tail lp), ls.
+  split.
+  { split.
+    { rewrite Happ. apply tail_app_l, Hnnil. }
+    by split; first apply no_commit_inv_commit.
+  }
+  by apply Forall_tail.
+Qed.
+(* TODO: move to invariance/commit *)
